verify commands
This also allows me to handle any invalid command easily

src/Commands.dfy
@@ -14,34 +14,41 @@ module Commands {
     | Guess(Maybe<seq<nat>>)
     | Stop(args:seq<string>)
 
+    // No post condition is required as we have checked the root methods.
     function stripColon(s : string) : Maybe<string>
+    requires |s| > 0  // Ensure string is non-empty for head operation
     {
       maybe(
-        head(s),
-        Nothing,
-        (res : char) =>
-        if res == ':'
-          then tail(s)
-          else Nothing
-        )
+      head(s),
+      Nothing,
+      (res : char) =>
+      if res == ':'
+        then tail(s)
+        else Nothing
+      )
     }
-
+    // Might not be necessary but for sanity sake I have added a precondition to match stripColon.
     function preprocess(s:string) : Maybe<(string,seq<string>)>
+    requires |s| > 0
     {
       maybe(stripColon(s), Nothing, (res : string) => splitCons(words(res)))
     }
 
     function processQuit(cmd : string, args : seq<string>) : Maybe<CMD>
+    ensures args != [] ==> processQuit(cmd, args) == Nothing  // If there are arguments, return Nothing
+    ensures cmd != "quit" ==> processQuit(cmd, args) == Nothing  // If command isn't "quit", return Nothing
+    ensures cmd == "quit" && args == [] ==> processQuit(cmd, args) == Just(Quit)  // Only allow quit with no args
     {
-      if cmd == "quit"
-        then Just(Quit)
-        else Nothing
+      if cmd == "quit" && args == []
+      then Just(Quit)
+      else Nothing
     }
 
     function processPlay(cmd : string, args : seq<string>) : Maybe<CMD>
     requires args != []
+    requires cmd == "play"
     {
-      if cmd == "play" && |args| == 2
+      if |args| == 2
         then
           var turns := stringToNat(args[0]);
           var sequence := digitsFromString(args[1]);
@@ -53,14 +60,14 @@ module Commands {
     requires args != []
     requires cmd == "guess"
     {
-      if cmd == "guess"
-        then
-          var guess := digitsFromString(args[0]);
-          Just(Guess(guess))
-        else Nothing
+      var guess := digitsFromString(args[0]);
+      Just(Guess(guess))
     }
 
     function processStop(cmd : string, args : seq<string>) : Maybe<CMD>
+    requires cmd == "stop"
+    ensures cmd != "stop" ==> processStop(cmd, args) == Nothing  // If command isn't "stop", return Nothing
+    ensures cmd == "stop" ==> processStop(cmd, args) == Just(Stop(args))  // If command is "stop", return Stop with args
     {
       if cmd == "stop"
         then Just(Stop(args))
@@ -68,6 +75,8 @@ module Commands {
     }
 
     function processHelp(cmd : string, args : seq<string>) : Maybe<CMD>
+    ensures cmd !in ["help", "h", "?"] ==> processHelp(cmd, args) == Nothing  // If command isn't help, return Nothing
+    ensures cmd in ["help", "h", "?"] ==> processHelp(cmd, args) == Just(Help)  // If command is help, return Help
     {
       if cmd in ["help", "h", "?"]
         then Just(Help)
@@ -77,19 +86,16 @@ module Commands {
 
     function process(cmd : string, args : seq<string>) : Maybe<CMD>
     {
-      whenNothing(
-      whenNothing(
-      whenNothing(
-      whenNothing(
-      processQuit(cmd, args),
-      processHelp(cmd, args)
-      ),
-      processPlay(cmd, args)
-      ),
-      processGuess(cmd, args)
-      ),
-      processStop(cmd, args)
-      )
+      if cmd == "play" && args != [] then
+        processPlay(cmd, args)
+      else if cmd == "guess" && args != [] then
+        processGuess(cmd, args)
+      else if cmd == "stop" then
+        processStop(cmd, args)
+      else if cmd == "quit" || cmd in ["help", "h", "?"] then
+        whenNothing(processQuit(cmd, args), processHelp(cmd, args))
+      else
+        Nothing
     }
 
     function fromString(s : string) : Maybe<CMD>
@@ -101,5 +107,4 @@ module Commands {
           process(res.0,res.1)
         )
     }
-
-}
+  }
